examples/proofs/tests/generated_spec.v
@@ -23,4 +23,8 @@ Section spec.
   (* Specifications for function [test_ternary]. *)
   Definition type_of_test_ternary :=
     fn(∀ () : (); True) → ∃ () : (), (void); True.
+
+  (* Specifications for function [test_bits]. *)
+  Definition type_of_test_bits :=
+    fn(∀ () : (); True) → ∃ () : (), (void); True.
 End spec.
